partial commit

safechecker/theories/PCUICEqualityDec.v
@@ -70,14 +70,17 @@ Definition compare_global_instance Σ equ lequ gr napp :=
 Definition eqb_binder_annots (x y : list aname) : bool :=
   forallb2 eqb_binder_annot x y.
 
-Fixpoint eqb_term_upto_univ_napp Σ (equ lequ : Universe.t -> Universe.t -> bool) napp (u v : term) : bool :=
+Fixpoint eqb_term_upto_univ_napp 
+  (equ lequ : Universe.t -> Universe.t -> bool) 
+  (gen_compare_global_instance : (Universe.t -> Universe.t -> bool) -> global_reference -> nat -> list Level.t -> list Level.t -> bool)
+  napp (u v : term) : bool :=
   match u, v with
   | tRel n, tRel m =>
     eqb n m
 
   | tEvar e args, tEvar e' args' =>
     eqb e e' &&
-    forallb2 (eqb_term_upto_univ_napp Σ equ equ 0) args args'
+    forallb2 (eqb_term_upto_univ_napp equ equ gen_compare_global_instance 0) args args'
 
   | tVar id, tVar id' =>
     eqb id id'
@@ -86,8 +89,8 @@ Fixpoint eqb_term_upto_univ_napp Σ (equ lequ : Universe.t -> Universe.t -> bool
     lequ u u'
 
   | tApp u v, tApp u' v' =>
-    eqb_term_upto_univ_napp Σ equ lequ (S napp) u u' &&
-    eqb_term_upto_univ_napp Σ equ equ 0 v v'
+    eqb_term_upto_univ_napp equ lequ gen_compare_global_instance (S napp) u u' &&
+    eqb_term_upto_univ_napp equ equ gen_compare_global_instance 0 v v'
 
   | tConst c u, tConst c' u' =>
     eqb c c' &&
@@ -95,52 +98,52 @@ Fixpoint eqb_term_upto_univ_napp Σ (equ lequ : Universe.t -> Universe.t -> bool
 
   | tInd i u, tInd i' u' =>
     eqb i i' &&
-    compare_global_instance Σ equ lequ (IndRef i) napp u u'
+    gen_compare_global_instance lequ (IndRef i) napp u u'
 
   | tConstruct i k u, tConstruct i' k' u' =>
     eqb i i' &&
     eqb k k' &&
-    compare_global_instance Σ equ lequ (ConstructRef i k) napp u u'
+    gen_compare_global_instance lequ (ConstructRef i k) napp u u'
 
   | tLambda na A t, tLambda na' A' t' =>
     eqb_binder_annot na na' &&
-    eqb_term_upto_univ_napp Σ equ equ 0 A A' &&
-    eqb_term_upto_univ_napp Σ equ lequ 0 t t'
+    eqb_term_upto_univ_napp equ equ gen_compare_global_instance 0 A A' &&
+    eqb_term_upto_univ_napp equ lequ gen_compare_global_instance 0 t t'
 
   | tProd na A B, tProd na' A' B' =>
     eqb_binder_annot na na' &&
-    eqb_term_upto_univ_napp Σ equ equ 0 A A' &&
-    eqb_term_upto_univ_napp Σ equ lequ 0 B B'
+    eqb_term_upto_univ_napp equ equ gen_compare_global_instance 0 A A' &&
+    eqb_term_upto_univ_napp equ lequ gen_compare_global_instance 0 B B'
 
   | tLetIn na B b u, tLetIn na' B' b' u' =>
     eqb_binder_annot na na' &&
-    eqb_term_upto_univ_napp Σ equ equ 0 B B' &&
-    eqb_term_upto_univ_napp Σ equ equ 0 b b' &&
-    eqb_term_upto_univ_napp Σ equ lequ 0 u u'
+    eqb_term_upto_univ_napp equ equ gen_compare_global_instance 0 B B' &&
+    eqb_term_upto_univ_napp equ equ gen_compare_global_instance 0 b b' &&
+    eqb_term_upto_univ_napp equ lequ gen_compare_global_instance 0 u u'
 
   | tCase indp p c brs, tCase indp' p' c' brs' =>
     eqb indp indp' &&
     eqb_predicate_gen
       (fun u u' => forallb2 equ (map Universe.make u) (map Universe.make u'))
       (bcompare_decls eqb eqb)
-      (eqb_term_upto_univ_napp Σ equ equ 0) p p' &&
-    eqb_term_upto_univ_napp Σ equ equ 0 c c' &&
+      (eqb_term_upto_univ_napp equ equ gen_compare_global_instance 0) p p' &&
+    eqb_term_upto_univ_napp equ equ gen_compare_global_instance 0 c c' &&
     forallb2 (fun x y =>
       forallb2 
         (bcompare_decls eqb eqb)
         x.(bcontext) y.(bcontext) &&
-      eqb_term_upto_univ_napp Σ equ equ 0 (bbody x) (bbody y)
+      eqb_term_upto_univ_napp equ equ gen_compare_global_instance 0 (bbody x) (bbody y)
     ) brs brs'
 
   | tProj p c, tProj p' c' =>
     eqb p p' &&
-    eqb_term_upto_univ_napp Σ equ equ 0 c c'
+    eqb_term_upto_univ_napp equ equ gen_compare_global_instance 0 c c'
 
   | tFix mfix idx, tFix mfix' idx' =>
     eqb idx idx' &&
     forallb2 (fun x y =>
-      eqb_term_upto_univ_napp Σ equ equ 0 x.(dtype) y.(dtype) &&
-      eqb_term_upto_univ_napp Σ equ equ 0 x.(dbody) y.(dbody) &&
+      eqb_term_upto_univ_napp equ equ gen_compare_global_instance 0 x.(dtype) y.(dtype) &&
+      eqb_term_upto_univ_napp equ equ gen_compare_global_instance 0 x.(dbody) y.(dbody) &&
       eqb x.(rarg) y.(rarg) &&
       eqb_binder_annot x.(dname) y.(dname)
     ) mfix mfix'
@@ -148,8 +151,8 @@ Fixpoint eqb_term_upto_univ_napp Σ (equ lequ : Universe.t -> Universe.t -> bool
   | tCoFix mfix idx, tCoFix mfix' idx' =>
     eqb idx idx' &&
     forallb2 (fun x y =>
-      eqb_term_upto_univ_napp Σ equ equ 0 x.(dtype) y.(dtype) &&
-      eqb_term_upto_univ_napp Σ equ equ 0 x.(dbody) y.(dbody) &&
+      eqb_term_upto_univ_napp equ equ gen_compare_global_instance 0 x.(dtype) y.(dtype) &&
+      eqb_term_upto_univ_napp equ equ gen_compare_global_instance 0 x.(dbody) y.(dbody) &&
       eqb x.(rarg) y.(rarg) &&
       eqb_binder_annot x.(dname) y.(dname)
     ) mfix mfix'
@@ -159,7 +162,8 @@ Fixpoint eqb_term_upto_univ_napp Σ (equ lequ : Universe.t -> Universe.t -> bool
   | _, _ => false
   end.
 
-Notation eqb_term_upto_univ Σ eq leq := (eqb_term_upto_univ_napp Σ eq leq 0).
+Notation eqb_term_upto_univ eq leq gen_compare_global_instance := 
+  (eqb_term_upto_univ_napp eq leq gen_compare_global_instance 0).
 
 Ltac eqspec :=
   lazymatch goal with
@@ -180,7 +184,7 @@ Local Ltac ih :=
   repeat lazymatch goal with
   | ih : forall lequ Rle napp hle t' ht ht', reflectT (eq_term_upto_univ_napp _ _ _ napp ?t _) _,
     hle : forall u u' hu hu', reflect (?Rle u u') (?lequ u u')
-    |- context [ eqb_term_upto_univ _ _ ?lequ ?t ?t' ] =>
+    |- context [ eqb_term_upto_univ _ ?lequ _ ?t ?t' ] =>
     destruct (ih lequ Rle 0 hle t') ; nodec ; subst
   end.
 
@@ -251,7 +255,9 @@ Proof.
   now move/andb_and: H => [].
 Qed.
 
-Lemma reflect_eq_context_IH {Σ equ lequ} {Re Rle : Universe.t -> Universe.t -> Prop} :
+Lemma reflect_eq_context_IH {Σ equ lequ} 
+  {Re Rle : Universe.t -> Universe.t -> Prop} 
+  {gen_compare_global_instance : (Universe.t -> Universe.t -> Prop) -> global_reference -> nat -> list Level.t -> list Level.t -> bool }:
   (forall u u', reflect (Re u u') (equ u u')) ->
   (forall u u', reflect (Rle u u') (lequ u u')) ->
   forall ctx ctx',
@@ -263,12 +269,12 @@ Lemma reflect_eq_context_IH {Σ equ lequ} {Re Rle : Universe.t -> Universe.t -> 
        (forall u u' : Universe.t, reflect (Rle u u') (lequ u u')) ->
        forall t' : term,
        reflectT (eq_term_upto_univ_napp Σ Re Rle napp t t')
-         (eqb_term_upto_univ_napp Σ equ lequ napp t t')) 
+         (eqb_term_upto_univ_napp equ lequ gen_compare_global_instance napp t t')) 
       ctx ->
   reflectT
     (eq_context_gen (eq_term_upto_univ Σ Re Re) (eq_term_upto_univ Σ Re Re) ctx ctx')
-    (forallb2 (bcompare_decls (eqb_term_upto_univ Σ equ equ)
-      (eqb_term_upto_univ Σ equ equ)) ctx ctx').
+    (forallb2 (bcompare_decls (eqb_term_upto_univ equ equ gen_compare_global_instance)
+      (eqb_term_upto_univ equ equ gen_compare_global_instance)) ctx ctx').
 Proof.
   intros hRe hRle ctx ctx' onc.
   eapply equiv_reflectT.
@@ -378,7 +384,9 @@ Proof.
     now apply /andP.
 Qed.
 
-Definition reflect_eq_predicate {Σ equ lequ} {Re Rle : Universe.t -> Universe.t -> Prop} {p : Universe.t -> bool} {q : nat -> term -> bool} :
+Definition reflect_eq_predicate {Σ equ lequ gen_compare_global_instance} {Re Rle : Universe.t -> Universe.t -> Prop}
+  {p : Universe.t -> bool} 
+  {q : nat -> term -> bool} :
   (forall u u', p u -> p u' -> reflect (Re u u') (equ u u')) ->
   (forall u u', p u -> p u' -> reflect (Rle u u') (lequ u u')) ->
   forall pr pr',
@@ -395,18 +403,18 @@ Definition reflect_eq_predicate {Σ equ lequ} {Re Rle : Universe.t -> Universe.t
    forall t' : term,
    on_universes p q t ->
    on_universes p q t' ->
-   reflectT (eq_term_upto_univ_napp Σ Re Rle napp t t') (eqb_term_upto_univ_napp Σ equ lequ napp t t'))
+   reflectT (eq_term_upto_univ_napp Σ Re Rle napp t t') (eqb_term_upto_univ_napp equ lequ gen_compare_global_instance napp t t'))
   (fun t : term =>
    forall (lequ : Universe.t -> Universe.t -> bool) (Rle : Universe.t -> Universe.t -> Prop) (napp : nat),
    (forall u u' : Universe.t, p u -> p u' -> reflect (Rle u u') (lequ u u')) ->
    forall t' : term,
    on_universes p q t ->
    on_universes p q t' ->
-   reflectT (eq_term_upto_univ_napp Σ Re Rle napp t t') (eqb_term_upto_univ_napp Σ equ lequ napp t t')) pr ->
+   reflectT (eq_term_upto_univ_napp Σ Re Rle napp t t') (eqb_term_upto_univ_napp equ lequ gen_compare_global_instance napp t t')) pr ->
   reflectT (eq_predicate (eq_term_upto_univ_napp Σ Re Re 0) Re pr pr') 
     (eqb_predicate_gen (fun u u' => forallb2 equ (map Universe.make u) (map Universe.make u'))
       (bcompare_decls eqb eqb)
-      (eqb_term_upto_univ_napp Σ equ equ 0) pr pr').
+      (eqb_term_upto_univ_napp equ equ gen_compare_global_instance 0) pr pr').
 Proof.
   intros.
   solve_all. unfold eq_predicate, eqb_predicate, eqb_predicate_gen.
@@ -439,7 +447,7 @@ Qed.
 
 Arguments eqb : simpl never.
 
-Lemma reflect_R_global_instance Σ equ lequ (p : Universe.t -> bool)
+Lemma reflect_R_global_instance Σ equ lequ  (p : Universe.t -> bool)
   (Re Rle : Universe.t -> Universe.t -> Prop) gr napp ui ui' :
   (forall u u', p u -> p u' -> reflect (Re u u') (equ u u')) ->
   (forall u u', p u -> p u' -> reflect (Rle u u') (lequ u u')) ->
@@ -490,7 +498,7 @@ Lemma reflect_eq_term_upto_univ Σ equ lequ
     on_universes p q t ->
     on_universes p q t' ->
     reflectT (eq_term_upto_univ_napp Σ Re Rle napp t t')
-             (eqb_term_upto_univ_napp Σ equ lequ napp t t').
+             (eqb_term_upto_univ_napp equ lequ (compare_global_instance Σ equ) napp t t').
 Proof.
   intros he hle t t' ht ht'.
   induction t in t', napp, lequ, Rle, hle, ht, ht' |- * using term_forall_list_ind.
@@ -517,15 +525,15 @@ Proof.
       * move: ht => /= /andP [? ?].
         move: ht' => /= /andP [? ?].
         destruct (p0 _ _ 0 he t) => //.
-        -- destruct (IHX l0) => //.
-           ++ constructor. constructor. constructor ; try assumption.
+        -- cbn.  destruct (IHX l0) => //.
+           ++ compute. constructor. constructor. constructor ; try assumption.
               inversion e0. subst. assumption.
            ++ constructor. intro bot. inversion bot. subst.
               inversion X0. subst.
               apply f. constructor. assumption.
         -- constructor. intro bot. apply f.
            inversion bot. subst. inversion X0. subst. assumption.
-  - cbn - [eqb]. eqspecs. equspec equ he. equspec lequ hle.
+  - cbn - [eqb]. equspec lequ hle.
     all: auto.
     ih.
     constructor. constructor. assumption.
@@ -713,7 +721,7 @@ Lemma eqb_term_upto_univ_impl (equ lequ : _ -> _ -> bool) Σ Re Rle napp:
   RelationClasses.subrelation lequ Rle ->
   RelationClasses.subrelation equ Rle ->
   forall t t',
-    eqb_term_upto_univ_napp Σ equ lequ napp t t' ->
+    eqb_term_upto_univ_napp equ lequ (compare_global_instance Σ equ) napp t t' ->
     eq_term_upto_univ_napp Σ Re Rle napp t t'.
 Proof.
   intros t t' he hle heqle.
@@ -743,7 +751,7 @@ Lemma eqb_term_upto_univ_refl :
   forall Σ (eqb leqb : Universe.t -> Universe.t -> bool) napp t,
     (forall u, eqb u u) ->
     (forall u, leqb u u) ->
-    eqb_term_upto_univ_napp Σ eqb leqb napp t t.
+    eqb_term_upto_univ_napp eqb leqb (compare_global_instance Σ eqb) napp t t.
 Proof.
   intros Σ eqb leqb napp t eqb_refl leqb_refl.
   case: (reflect_eq_term_upto_univ Σ eqb leqb xpredT (fun _ => xpredT) eqb leqb napp _ _ t t) => //.
@@ -751,6 +759,21 @@ Proof.
   1-2: apply on_universes_true.
   now unshelve epose proof (eq_term_upto_univ_refl Σ eqb leqb napp _ _ t).
 Qed.
+
+(* genereic equality for contexts *)
+
+Fixpoint eqb_ctx_gen equ gen_compare_global_instance
+    (Γ Δ : context) : bool :=
+    match Γ, Δ with
+    | [], [] => true
+    | {| decl_name := na1 ; decl_body := None ; decl_type := t1 |} :: Γ,
+      {| decl_name := na2 ; decl_body := None ; decl_type := t2 |} :: Δ =>
+      eqb_binder_annot na1 na2 && eqb_term_upto_univ equ equ gen_compare_global_instance t1 t2  && eqb_ctx_gen equ gen_compare_global_instance Γ Δ
+    | {| decl_name := na1 ; decl_body := Some b1 ; decl_type := t1 |} :: Γ,
+      {| decl_name := na2 ; decl_body := Some b2 ; decl_type := t2 |} :: Δ =>
+      eqb_binder_annot na1 na2 && eqb_term_upto_univ equ equ gen_compare_global_instance b1 b2 && eqb_term_upto_univ equ equ gen_compare_global_instance t1 t2 && eqb_ctx_gen equ gen_compare_global_instance Γ Δ
+    | _, _ => false
+    end.
 
 (** Checking equality *)
 
@@ -765,14 +788,26 @@ Section EqualityDec.
     destruct hΣ, Hφ; now constructor.
   Defined.
 
+
+  Definition conv_pb_relb_gen pb (eq leq : Universe.t -> Universe.t -> bool) :=
+    match pb with
+    | Conv => eq
+    | Cumul => leq
+    end.
+  
   Definition conv_pb_relb pb :=
     match pb with
     | Conv => check_eqb_universe G
     | Cumul => check_leqb_universe G
     end.
-  
-  Definition eqb_termp_napp pb napp :=
-    eqb_term_upto_univ_napp Σ (check_eqb_universe G) (conv_pb_relb pb) napp.
+
+  Definition eqb_termp_napp_gen pb eq leq compare_global_instance_gen napp :=
+      eqb_term_upto_univ_napp eq (conv_pb_relb_gen pb eq leq) 
+                compare_global_instance_gen napp.
+
+  Definition eqb_termp_napp pb :=
+    eqb_termp_napp_gen pb (check_eqb_universe G) (check_leqb_universe G) 
+          (compare_global_instance Σ (check_eqb_universe G)).
 
     Lemma eq_universeP u u' :
     wf_universe Σ u ->
@@ -922,17 +957,7 @@ Section EqualityDec.
     all: apply check_eqb_universe_refl.
   Qed.
 
-  Fixpoint eqb_ctx (Γ Δ : context) : bool :=
-    match Γ, Δ with
-    | [], [] => true
-    | {| decl_name := na1 ; decl_body := None ; decl_type := t1 |} :: Γ,
-      {| decl_name := na2 ; decl_body := None ; decl_type := t2 |} :: Δ =>
-      eqb_binder_annot na1 na2 && eqb_term t1 t2 && eqb_ctx Γ Δ
-    | {| decl_name := na1 ; decl_body := Some b1 ; decl_type := t1 |} :: Γ,
-      {| decl_name := na2 ; decl_body := Some b2 ; decl_type := t2 |} :: Δ =>
-      eqb_binder_annot na1 na2 && eqb_term b1 b2 && eqb_term t1 t2 && eqb_ctx Γ Δ
-    | _, _ => false
-    end.
+  Definition eqb_ctx := eqb_ctx_gen (check_eqb_universe G) (compare_global_instance Σ (check_eqb_universe G)).
 
   Lemma eqb_binder_annot_spec {A} na na' : eqb_binder_annot (A:=A) na na' -> eq_binder_annot (A:=A) na na'.
   Proof. case: eqb_annot_reflect => //. Qed.
