safechecker/theories/PCUICWfEnv.v
@@ -5,6 +5,48 @@ From MetaCoq.Template Require Import config utils uGraph.
 From MetaCoq.PCUIC Require Import PCUICAst PCUICAstUtils
      PCUICReflect PCUICTyping PCUICGlobalEnv.
      
+From MetaCoq.SafeChecker Require Import PCUICEqualityDec.
+(* We pack up all the information required on the global environment and graph in a 
+   single record. *)
+
+Class wf_env_struct {cf:checker_flags} (wf_env_impl : Type) := {
+  wf_env_lookup : wf_env_impl -> kername -> option global_decl;
+  wf_env_eq : wf_env_impl -> Universe.t -> Universe.t -> bool;
+  wf_env_leq : wf_env_impl -> Universe.t -> Universe.t -> bool;
+  wf_env_compare_global_instance : wf_env_impl -> (Universe.t -> Universe.t -> bool) -> global_reference -> nat -> list Level.t -> list Level.t -> bool;
+  (* This part of the structure is here to state the correctness properties *)
+  wf_env_env : wf_env_impl -> global_env_ext ;
+  wf_env_graph : wf_env_impl -> universes_graph;
+}.
+
+Class wf_env_prop {cf:checker_flags} (wf_env_impl : Type) (X : wf_env_struct wf_env_impl) : Prop := {
+  wf_env_wf X : ∥ wf_ext (wf_env_env X) ∥;
+  wf_env_lookup_correct X c : 
+    lookup_env (wf_env_env X) c = wf_env_lookup X c ;
+  wf_env_eq_correct X : check_eqb_universe (wf_env_graph X) = wf_env_eq X;
+  wf_env_leq_correct X : check_leqb_universe (wf_env_graph X) = wf_env_leq X;
+  wf_env_compare_global_instance_correct X : 
+    compare_global_instance (wf_env_env X) (check_eqb_universe (wf_env_graph X)) = 
+    wf_env_compare_global_instance X;
+  wf_env_graph_wf X : 
+      is_graph_of_uctx (wf_env_graph X) (global_ext_uctx (wf_env_env X))
+   }.
+
+Definition wf_env_impl {cf:checker_flags} := ∑ X Y, wf_env_prop X Y. 
+
+Global Instance wf_env_impl_wf_env_struct {cf:checker_flags} (Σ : wf_env_impl) : wf_env_struct Σ.π1.
+  exact (Σ.π2.π1).
+Defined. 
+
+Global Instance wf_env_impl_wf_env_prop {cf:checker_flags} (Σ : wf_env_impl) : wf_env_prop Σ.π1 _.
+  exact (Σ.π2.π2).
+Defined. 
+
+Definition wf_env_ext_sq_wf {cf:checker_flags} (Σ : wf_env_impl) (x : Σ.π1) : ∥ wf (wf_env_env x) ∥.
+  destruct (wf_env_wf x).
+  sq. auto. 
+Qed.
+
 Lemma wf_ext_gc_of_uctx {cf:checker_flags} {Σ : global_env_ext} (HΣ : ∥ wf_ext Σ ∥)
   : ∑ uctx', gc_of_uctx (global_ext_uctx Σ) = Some uctx'.
 Proof.
